TAPLFormalization/02-lambda/Programming.lean
@@ -1,5 +1,6 @@
 import TAPLFormalization.«02-lambda».Semantics
 import TAPLFormalization.«02-lambda».SemanticsTheorems
+import TAPLFormalization.«01-peano».Semantics
 
 infixl:100 "|$|" => LambdaTerm.app
 abbrev la := LambdaTerm.abs
@@ -13,6 +14,7 @@ def cNot : LambdaTerm := la "b" $ la "x" $ la "y" $ "b" |$| "y" |$| "x"
 def cOr : LambdaTerm := la "a" $ la "b" $ "a" |$| cTrue |$| ("b" |$| cTrue |$| cFalse)
 def cAnd : LambdaTerm := la "a" $ la "b" $ "a" |$| ("b" |$| cTrue |$| cFalse) |$| cFalse
 def cTest : LambdaTerm := la "l" $ la "m" $ la "n" $ "l" |$| "m" |$| "n"
+def cBoolEval (t : LambdaTerm) : LambdaTerm := t |$| la "x" "true" |$| la "x" "false"
 
 def cPair : LambdaTerm := la "f" $ la "s" $ la "b" $ "b" |$| "f" |$| "s"
 def cFst : LambdaTerm := la "p" $ "p" |$| cTrue
@@ -29,24 +31,47 @@ def _ss : LambdaTerm := la "p" $ cPair |$| (cSnd |$| "p") |$| (cPlus |$| (cNum 1
 def cPred : LambdaTerm := la "m" $ cFst |$| ("m" |$| _ss |$| _zz)
 def cSub : LambdaTerm := la "n" $ la "m" $ "n" |$| cPred |$| "m"
 def cEq : LambdaTerm := la "n" $ la "m" $ cAnd |$| (cIsZro |$| (cSub |$| "m" |$| "n")) |$| (cIsZro |$| (cSub |$| "n" |$| "m"))
-#eval CV.getNF 410 (removeNames $ cEq |$| (cPred |$| cNum 4) |$| (cNum 3) |$| la "x" "true" |$| la "x" "false")
+#eval CallByValue.run 410 (removeNames $ cEq |$| (cPred |$| cNum 4) |$| (cNum 3) |$| la "x" "true" |$| la "x" "false")
 
-infix:100 " ~> " => CV.SmallStep
 def cId : LambdaTerm := la "x" "x"
 
 def test1 := removeNames (cFst |$| (cPair |$| la "" "v" |$| la "" "w"))
-def res := CV.getNF 10 test1
+def res := CallByValue.run 10 test1
 #eval res
 
 def test2 := removeNames $ cId |$| (cId |$| (la "z" (cId |$| "z")))
-example : CV.SmallSteps (removeNames $ cId |$| (cId |$| (la "z" (cId |$| "z")))) (removeNames $ la "z" $ cId |$| "z") := by
+example : (removeNames $ cId |$| (cId |$| (la "z" (cId |$| "z")))) ~cbv~>* (removeNames $ la "z" $ cId |$| "z") := by
   calc
-    _ ~> (removeNames $ cId |$| (la "z" (cId |$| "z"))) := by
+    _ ~cbv~> (removeNames $ cId |$| (la "z" (cId |$| "z"))) := by
       simp [removeNames, removeNames', cId]
       apply CV.SmallStep.appArg
       apply CV.SmallStep.appAbs
       simp [subst, subst', addDepth]
-    _ ~> _ := by
+    _ ~cbv~> _ := by
       simp [removeNames, removeNames', cId]
       apply CV.SmallStep.appAbs
       simp [subst, subst', addDepth]
+
+def test3 := cTrue |$| cTrue |$| cFalse
+#eval CallByValue.run 2 (removeNames test3)
+
+-- R lt bt → ∃ lz bz, LSteps lt lz ∧ isValue lz ∧ R lz bz ∧ BSteps bt bz
+-- R lt bt → R lz bz → LSteps lt lz → BSteps bt bz
+
+-- def embed' : Term → LambdaTerm
+--   | .trueV => cTrue
+--   | .falseV => cFalse
+--   | .zero => cZero
+--   | .ifThenElse c t e => cTest |$| (embed' c) |$| (embed' t) |$| (embed' e)
+--   | .succ t => cSucc |$| embed' t
+--   | .pred t => cPred |$| embed' t
+--   | .isZero t => cIsZro |$| embed' t
+
+-- def embed := removeNames ∘ embed'
+
+-- def lambda_steps_of_peano_step : BooleanTerm t → t ~> t' → (removeNames $ cBoolEval $ embed' t) ~>λ (removeNames $ cBoolEval $ embed' t') := by
+--   intro t_bool term_st
+--   induction term_st <;> try grind [Term, BooleanTerm]
+--   case IfTrue t e =>
+--     simp [embed', removeNames, removeNames', cBoolEval, cTest, Std.HashMap.getElem_insert]
+--   sorry
