TAPLFormalization/02-lambda/SemanticsEquivalence.lean
@@ -1,0 +1,79 @@
+import TAPLFormalization.«01-peano».Semantics
+import TAPLFormalization.«02-lambda».Programming
+
+-- BR lt bt: lt is equivalent to a purely boolean term bt
+inductive BR : IndexedTerm → Term → Prop where
+  | trueV : BR (.abs (.abs (.boundV 0))) .trueV
+  | falseV : BR (.abs (.abs (.boundV 1))) .falseV
+  | cond : BR lc bc → BR lt bt → BR le be → BR (.app (.app lc lt) le) (.ifThenElse bc bt be)
+
+lemma br_deterministic : BR lt bt → BR lt' bt → lt = lt' := by
+  intro r r'
+  induction r' generalizing lt <;> grind [BR]
+
+lemma br_defined : BooleanTerm bt → ∃ lt, BR lt bt := by
+  intro bt_bt
+  induction bt <;> cases bt_bt
+  · exact ⟨_, by constructor⟩
+  · exact ⟨_, by constructor⟩
+  · rename_i c t e c_ih t_ih e_ih c_bt t_bt e_bt
+    let ⟨lc, r_c⟩ := c_ih c_bt
+    let ⟨lt, r_t⟩ := t_ih t_bt
+    let ⟨le, r_e⟩ := e_ih e_bt
+    exists (.app (.app lc lt) le)
+    constructor <;> assumption
+
+lemma bt_of_br : BR lt bt → BooleanTerm bt := by
+  intro br
+  induction br <;> grind [BooleanTerm]
+
+lemma step_preserves_bt : BooleanTerm t₁ → t₁ ~> t₂ → BooleanTerm t₂ := by
+  intro t₁_bt st
+  induction st <;> cases t₁_bt <;> grind [BooleanTerm]
+
+lemma subst_addDepth : subst t₁ (addDepth 1 t₂) = t₂ := by
+  rw [subst]
+  generalize 0 = k
+  induction t₂ generalizing k <;> grind [subst', addDepth]
+
+lemma addDepth_zero : addDepth 0 t = t := by
+  induction t <;> grind [addDepth]
+
+lemma soundness_ltob_single : BR lt bt → BR lz bz → bt ~> bz → lt ~no~>* lz := by
+  intro lt_r_bt lz_r_bz b_st
+  induction lt_r_bt generalizing lz bz <;> cases b_st
+  case IfTrue lc lt bt le be t_r e_r t_ih e_ih c_r _ =>
+    cases c_r
+    let lz_eq := br_deterministic lz_r_bz t_r
+    rw [lz_eq]
+    calc
+      _ ~no~> .app (.abs (addDepth 1 lt)) le := .appBody (.appAbs (by simp [subst, subst']))
+      _ ~no~> _ := .appAbs (by rw [subst_addDepth])
+  case IfFalse lc lt bt le be t_r e_r t_ih e_ih c_r _ =>
+    cases c_r
+    let lz_eq := br_deterministic lz_r_bz e_r
+    rw [lz_eq]
+    calc
+      _ ~no~> .app (.abs (.boundV 0)) le := .appBody (.appAbs (by simp [subst, subst']))
+      _ ~no~> _ := .appAbs (by rw [subst, subst', addDepth_zero])
+  case If lc bc lt bt le be c_r t_r e_r c_ih t_ih e_ih bc' st =>
+    cases lz_r_bz with
+    | cond c'_r t'_r e'_r =>
+      let c_sts := c_ih c'_r st
+      let lt_eq := br_deterministic t'_r t_r
+      let le_eq := br_deterministic e'_r e_r
+      rw [lt_eq, le_eq]
+      let f (t : IndexedTerm) := IndexedTerm.app (.app t lt) le
+      let cons {t₁ t₂ : IndexedTerm} (st : t₁ ~no~> t₂) : (f t₁) ~no~> (f t₂) :=
+        NO.SmallStep.appBody (NO.SmallStep.appBody st)
+      apply ReflTransGen'.lift f cons c_sts
+
+theorem soundness_ltob : BR lt bt → BR lz bz → bt ~>* bz → lt ~no~>* lz := by
+  intro lt_r_bt lz_r_bz b_sts
+  induction b_sts generalizing lt lz
+  case refl => grind [br_deterministic, ReflTransGen']
+  case tail bt bt' bz b_st b_sts' ih =>
+    let ⟨lt', lt'_r_bt'⟩ := br_defined (step_preserves_bt (bt_of_br lt_r_bt) b_st)
+    let l_sts' := ih lt'_r_bt' lz_r_bz
+    apply ReflTransGen'.trans ?_ l_sts'
+    exact soundness_ltob_single lt_r_bt lt'_r_bt' b_st
